yalla/bbb.v
@@ -12,9 +12,7 @@ Require Import List_Type_more.
 Require Import Permutation_Type_more.
 Require Import Permutation_Type_solve.
 Require Import genperm_Type.
-Require Import Forall_Type_more2.
 Require Import Dependent_Forall_Type.
-Require Import concat_Type_more.
 Require Import Eqdep_dec.
 
 Require Import ll_fragments.
@@ -175,7 +173,7 @@ induction H using (ll_nested_ind _); try now constructor.
   simpl; rewrite app_nil_r.
   assert (ll_bbb l1) as pi1.
   { destruct (In_Forall_Type_in _ _ _ PL (in_Type_elt l1 (l0 :: nil) nil)) as (pi & Hin).
-    refine (Dependent_Forall_Type_in (list_eq_dec formula_eq_dec) _ _ PL _ _ X Hin). }
+    refine (Dependent_Forall_Type_forall (list_eq_dec formula_eq_dec) _ _ _ _ PL X Hin). }
   inversion PL; inversion X1; subst; clear X1 X2 X3.
   apply mix2_bbb_r...
   eapply stronger_pfrag...
@@ -633,11 +631,11 @@ induction pi using (ll_nested_ind _); try now econstructor.
   + assert (In_Type l1 (l0 :: l1 :: nil)) as Hin.
     { right; left... }
     apply (In_Forall_Type_in _ _ _ PL) in Hin as (pi & Hin).
-    refine (Dependent_Forall_Type_in (list_eq_dec formula_eq_dec) _ _ PL _ _ X Hin).
+    refine (Dependent_Forall_Type_forall (list_eq_dec formula_eq_dec) _ _ _ _ PL X Hin).
   + assert (In_Type l0 (l0 :: l1 :: nil)) as Hin.
     { left... }
     apply (In_Forall_Type_in _ _ _ PL) in Hin as (pi & Hin).
-    refine (Dependent_Forall_Type_in (list_eq_dec formula_eq_dec) _ _ PL _ _ X Hin).
+    refine (Dependent_Forall_Type_forall (list_eq_dec formula_eq_dec) _ _ _ _ PL X Hin).
 Qed.
 
 Theorem bb_to_bbb : forall l, llR (oc bot) l -> ll_bbb l.
