yalla/nn_def.v
@@ -8,9 +8,7 @@ Require Import List_more.
 Require Import List_Type_more.
 Require Import Permutation_Type.
 Require Import genperm_Type.
-Require Import Forall_Type_more2.
 Require Import Dependent_Forall_Type.
-Require Import concat_Type_more.
 
 Require Import subs.
 Require Import isubs.
